src/subgroup/composition.lean
@@ -1,0 +1,196 @@
+import subgroup.torsion
+
+open_locale classical
+
+namespace mygroup
+
+open mygroup mygroup.subgroup mygroup.quotient group_hom function set
+
+/-- A group is nontrivial if and only if it top is not equal to its bot -/
+def group.nontrivial (G : Type) [group G] : Prop := (⊥ : subgroup G) ≠ ⊤ 
+
+@[simp] lemma group.nontrivial_def {G : Type} [group G] :
+  group.nontrivial G ↔ (⊥ : subgroup G) ≠ ⊤ := iff.rfl
+
+-- Some lemmas about pushing top and bot over isomorphisms
+lemma subgroup.iso_bot_eq_bot {G H : Type} [group G] [group H] 
+  (φ : G ≅ H) : subgroup.map φ.1 (⊥ : subgroup G) = (⊥ : subgroup H) := 
+begin
+  ext, rw [mem_map, mem_bot_iff],
+  split, 
+    { rintro ⟨_, hx, rfl⟩,
+      rw mem_bot_iff at hx,
+      subst hx,
+      exact map_one _ },
+    { rintro rfl,
+      exact ⟨1, mem_bot_iff.2 rfl, map_one _⟩ }
+end
+
+/-- Everything is a member of top -/
+lemma subgroup.mem_top {G : Type} [group G] (g : G) : g ∈ (⊤ : subgroup G) :=
+begin
+  change g ∈ ((⊤ : subgroup G) : set G),
+  rw ← singleton_subset_iff,
+  change {g} ≤ ((⊤ : subgroup G) : set G),
+  rw ← subgroup.closure_le, simp,
+end
+
+lemma subgroup.iso_top_eq_top {G H : Type} [group G] [group H] 
+  (φ : G ≅ H) : subgroup.map φ.1 (⊤ : subgroup G) = (⊤ : subgroup H) := 
+begin
+  ext, split; intro,
+    { exact subgroup.mem_top _ },
+    { rw mem_map,
+      rcases φ.2.2 x with ⟨x, rfl⟩,
+      refine ⟨x, subgroup.mem_top _, rfl⟩ }
+end
+
+/-- Nontrivial is a group property, that is it translates over group isomorphisms -/
+lemma subgroup.nontrivial_of_iso_nontrivial {G H : Type} [group G] [group H] 
+  (φ : G ≅ H) : group.nontrivial G → group.nontrivial H :=
+begin
+  intros hG h,
+  apply hG, 
+  rw [← subgroup.iso_top_eq_top (iso_symm φ),
+      ← subgroup.iso_bot_eq_bot (iso_symm φ), h],
+end
+
+namespace normal
+
+variables {G : Type} [group G]
+
+-- def subgroup.le_hom {A B : subgroup G} (hAB : A ≤ B) : A →* B :=
+--   monoid_hom.mk' (λ a, ⟨a.1, hAB a.2⟩) (λ _ _, rfl)
+
+-- def subgroup.normal_pair {A B : subgroup G} (hAB : A ≤ B) : Prop :=
+--   (monoid_hom.range (subgroup.le_hom hAB)).normal
+
+-- @[simp] lemma subgroup.normal_pair_def {A B : subgroup G} (hAB : A ≤ B) :
+--   subgroup.normal_pair hAB ↔ (monoid_hom.range (subgroup.le_hom hAB)).normal := iff.rfl
+
+-- def subgroup.normal_pair' (A B : subgroup G): Prop :=
+--   (monoid_hom.range (subgroup.le_hom (show A ⊓ B ≤ B, by exact inf_le_right))).normal
+
+-- instance : has_top $ normal G := 
+-- ⟨ { carrier := univ,
+--     one_mem' := mem_univ _,
+--     mul_mem' := λ _ _ _ _, mem_univ _,
+--     inv_mem' := λ _ _, mem_univ _,
+--     conj_mem' := λ _ _ _, mem_univ _ } ⟩
+
+/-- The normal subgroup of a normal subgroup induced by a smaller normal 
+  subgroup through the inclusion map -/
+def normal.𝒾 {G : Type} [group G] {A B : normal G} (hle : A ≤ B) : normal B :=
+{ carrier := { b | b.1 ∈ A },
+  one_mem' := A.one_mem',
+  mul_mem' := λ _ _ ha hb, A.mul_mem' ha hb,
+  inv_mem' := λ _ h, A.inv_mem' h,
+  conj_mem' := λ _ h _, A.conj_mem' _ h _ }
+
+variables (H : subgroup G) (N : normal G)
+
+/-- A group is simple if and only if it is nontrivial and all its normal subgroups 
+  are either top or bot -/
+def is_simple (G : Type) [group G] :=
+  group.nontrivial G ∧ ∀ N : normal G, N = ⊥ ∨ N = ⊤
+
+@[simp] lemma is_simple_def (G : Type) [group G] : is_simple G ↔ 
+  group.nontrivial G ∧ ∀ N : normal G, N = ⊥ ∨ N = ⊤ := iff.rfl
+
+def chain_prop (A B : normal G) : Prop :=
+  ∃ (hle : A ≤ B), is_simple $ B /ₘ (normal.𝒾 hle)
+
+@[simp] lemma chain_prop_def {A B : normal G} :
+  chain_prop A B ↔ 
+  ∃ (hle : A ≤ B), is_simple $ B /ₘ (normal.𝒾 hle) := iff.rfl
+
+instance normal.inhabited : inhabited $ normal G := ⟨ ⊥ ⟩
+
+/-- Chain is a nonempty list of normal subgroups such that subsequent subgroups 
+  satisfies `chain_prop`, and furthermore, it begins with bot and ends with top -/
+structure chain (G : Type) [group G] :=
+(carrier    : list (normal G))
+(nonempty   : carrier ≠ list.nil)
+(chain_prop : carrier.chain' chain_prop)
+(chain_head : carrier.head = ⊥)
+(chain_last : carrier.last nonempty = ⊤)
+
+/-- A normal subgroup is maximal if and only if the quotient group by it is 
+  simple -/
+def is_maximal {N : normal G} (hN : N ≠ ⊤) : Prop := is_simple (G /ₘ N)
+
+@[simp] lemma is_maximal_def {N : normal G} (hN : N ≠ ⊤) : 
+  is_maximal hN ↔ is_simple (G /ₘ N) := iff.rfl
+
+-- If N < M, then by the correspondence theorem, there is a proper normal 
+-- subgroup in G / N which contradicts the is_simple hypothesis
+
+/-- There is no proper subgroup containing a maximal subgroup -/
+theorem maximal_is_max {N : normal G} (hproper : N ≠ ⊤) (h : is_maximal hproper) : 
+  ∀ M : normal G, N < M → M = ⊤ :=
+begin
+  intros M hM,
+  rw [is_maximal_def, is_simple_def] at h,
+  rcases h with ⟨h₁, h₂⟩,
+  cases h₂ ((normal_of_quotient_order_iso N).to_equiv ⟨M, le_of_lt hM⟩),
+    { exfalso, refine not_le_of_lt hM _,
+      change (⟨M, le_of_lt hM⟩ : { H // N ≤ H }) ≤ ⟨N, le_refl _⟩, 
+      rw [(normal_of_quotient_order_iso N).ord', h],
+      exact bot_le },
+    { rw eq_top_iff,
+      change (⟨⊤, le_top⟩ : { H // N ≤ H }) ≤ ⟨M, le_of_lt hM⟩, 
+      rw [(normal_of_quotient_order_iso N).ord', h],
+      exact le_top }
+end
+
+/-- An alternative version of `maximal_is_max` that requires `≤` instead of `<` -/
+theorem maximal_is_max' {N : normal G} (hproper : N ≠ ⊤) (h : is_maximal hproper) : 
+  ∀ M : normal G, N ≤ M → M = N ∨ M = ⊤ := 
+begin
+  intros M hM,
+  rcases le_iff_lt_or_eq.1 hM with hlt | rfl,
+    { exact or.inr (maximal_is_max hproper h _ hlt) },
+    { exact or.inl rfl }
+end
+
+/-- Everything is in top -/
+lemma mem_top {G : Type} [group G] (g : G) : g ∈ (⊤ : normal G) :=
+begin
+  rw [← mem_carrier, ← singleton_subset_iff],
+  change {g} ≤ ((⊤ : normal G) : set G),
+  rw ← normal.closure_le, simp,
+end
+
+def top_div_bot_iso : 
+  G ≅ (⊤ : normal G) /ₘ (@normal.𝒾 _ _ ⊥ (⊤ : normal G) le_top) :=
+{ to_fun := λ g, quotient.mk (@normal.𝒾 _ _ ⊥ (⊤ : normal G) le_top) 
+    (⟨g, mem_top _⟩ : (⊤ : normal G)),
+  map_mul' := sorry,
+  is_bijective := sorry }
+
+def trivial_chain (h : is_simple G) (hG : group.nontrivial G) : chain G := 
+{ carrier := [⊥, ⊤],
+  nonempty := by simp,
+  chain_prop := 
+    begin
+      simp, 
+      refine ⟨subgroup.nontrivial_of_iso_nontrivial (top_div_bot_iso) hG, _⟩,
+        { sorry }
+    end,
+  chain_head := by simp,
+  chain_last := by simp }
+
+example [fintype G] : ∀ (n = fintype.card G), ∃ c : chain G, true :=
+begin
+  intro n, apply nat.strong_induction_on n,
+  rintros k hk₁ rfl,
+  by_cases is_simple G,
+    sorry,
+    sorry
+end
+
+instance [fintype G] : inhabited $ chain G := ⟨ sorry ⟩
+
+end normal
+
+end mygroup
